SoftwareFoundations/ProgrammingLanguageFoundations/Equiv.lean
@@ -81,7 +81,7 @@ namespace SoftwareFoundations.ProgrammingLanguageFoundations.Equiv
     False.elim (by simp_all)
 
   namespace Term
-    theorem Command.skip_left {c: Command}: [Imp| skip; <[c]>] ≈ c
+    theorem Command.skip_left {c: Command}: [Imp| skip; ‹c›] ≈ c
       | _, _ =>
         have mp
           | .seq _ _ _ (.skip _) h₂ => h₂
@@ -95,7 +95,7 @@ namespace SoftwareFoundations.ProgrammingLanguageFoundations.Equiv
           | .whileFalse _ h₁          => .seq _ _ _ (.skip _) (.whileFalse _ h₁)
         ⟨mp, mpr⟩
 
-    theorem Command.skip_right {c: Command}: [Imp| <[c]>; skip] ≈ c
+    theorem Command.skip_right {c: Command}: [Imp| ‹c›; skip] ≈ c
       | _, _ =>
         have mp
           | .seq _ _ _ h₁ (.skip _) => h₁
@@ -109,7 +109,7 @@ namespace SoftwareFoundations.ProgrammingLanguageFoundations.Equiv
           | .whileFalse _ h₁          => .seq _ _ _ (.whileFalse _ h₁) (.skip _)
         ⟨mp, mpr⟩
 
-    example {t f: Command}: [Imp| ite (tru) { <[t]> } else { <[f]> }] ≈ t
+    example {t f: Command}: [Imp| ite (tru) { ‹t› } else { ‹f› }] ≈ t
       | _, _ =>
         have mp
           | .ifTrue _ _ _ h₂ => h₂
@@ -124,7 +124,7 @@ namespace SoftwareFoundations.ProgrammingLanguageFoundations.Equiv
           | .whileFalse _ h           => .ifTrue _ _ rfl (.whileFalse _ h)
         ⟨mp, mpr⟩
 
-    theorem Command.if_true {b: Logic} {c₁ c₂: Command} (h: b ≈ .true): [Imp| ite (<[b]>) { <[ c₁ ]> } else { <[ c₂ ]> }] ≈ c₁
+    theorem Command.if_true {b: Logic} {c₁ c₂: Command} (h: b ≈ .true): [Imp| ite (‹b›) { ‹c₁› } else { ‹c₂› }] ≈ c₁
       | _, _ =>
         have truu: b.eval _ = Logic.true.eval _ := h _
         have mp
@@ -140,7 +140,7 @@ namespace SoftwareFoundations.ProgrammingLanguageFoundations.Equiv
           | .whileFalse _ h₁          => .ifTrue _ _ truu (.whileFalse _ h₁)
         ⟨mp, mpr⟩
 
-    theorem Command.if_false {b: Logic} {c₁ c₂: Command} (h: b ≈ .false): [Imp| ite (<[b]>) { <[ c₁ ]> } else { <[ c₂ ]> }] ≈ c₂
+    theorem Command.if_false {b: Logic} {c₁ c₂: Command} (h: b ≈ .false): [Imp| ite (‹b›) { ‹c₁› } else { ‹c₂› }] ≈ c₂
       | _, _ =>
         have falz: b.eval _ = Logic.false.eval _ := h _
         have mp
@@ -156,13 +156,13 @@ namespace SoftwareFoundations.ProgrammingLanguageFoundations.Equiv
           | .whileFalse _ h₁          => .ifFalse _ _ falz (.whileFalse _ h₁)
         ⟨mp, mpr⟩
 
-    theorem Command.if_swap {b: Logic} {c₁ c₂: Command}: [Imp| ite (<[b]>) { <[ c₁ ]> } else { <[ c₂ ]> }] ≈ [Imp| ite ( ! <[b]> ) { <[ c₂ ]> } else { <[ c₁ ]> }]
+    theorem Command.if_swap {b: Logic} {c₁ c₂: Command}: [Imp| ite (‹b›) { ‹c₁› } else { ‹c₂› }] ≈ [Imp| ite ( ! ‹b› ) { ‹c₂› } else { ‹c₁› }]
       | _, _ =>
         have mp := sorry
         have mpr := sorry
         ⟨mp, mpr⟩
 
-    theorem Command.while_false {c: Logic} {b: Command} (h: c ≈ .false): [Imp| while (<[c]>) { <[b]> }] ≈ [Imp| skip]
+    theorem Command.while_false {c: Logic} {b: Command} (h: c ≈ .false): [Imp| while (‹c›) { ‹b› }] ≈ [Imp| skip]
       | _, _ =>
         have falz: c.eval _ = Logic.false.eval _ := h _
         have mp
@@ -172,7 +172,7 @@ namespace SoftwareFoundations.ProgrammingLanguageFoundations.Equiv
           | .skip _ => .whileFalse _ falz
         ⟨mp, mpr⟩
 
-    theorem Command.while_true {c: Logic} {b: Command} (h: c ≈ .true): [Imp| while (<[c]>) { <[b]> }] ≈ [Imp| while (tru) { skip }]
+    theorem Command.while_true {c: Logic} {b: Command} (h: c ≈ .true): [Imp| while (‹c›) { ‹b› }] ≈ [Imp| while (tru) { skip }]
       | _, _ =>
         have truu: c.eval _ = Logic.true.eval _ := h _
         have hh: Logic.true.equiv .true
@@ -185,12 +185,12 @@ namespace SoftwareFoundations.ProgrammingLanguageFoundations.Equiv
           | .whileFalse _ h₁ => Logic.true.trueFalse rfl h₁
         ⟨mp, mpr⟩
       where
-        nonterm {c: Logic} {b: Command} {s₁ s₂: State} (h: c ≈ .true): ¬(s₁ =[[Imp| while (<[c]>) { <[b]> }]]=> s₂)
+        nonterm {c: Logic} {b: Command} {s₁ s₂: State} (h: c ≈ .true): ¬(s₁ =[[Imp| while (‹c›) { ‹b› }]]=> s₂)
           | .whileTrue s₁ s₂ s₃ h₁ h₂ h₃ =>
             sorry
           | .whileFalse _ h₁ => c.trueFalse (h _) h₁
 
-    theorem Command.loop_unrolling {c: Logic} {b: Command}: [Imp| while (<[c]>) { <[b]> }] ≈ [Imp| ite (<[c]>) { <[b]>; while (<[c]>) { <[b]> }} else { skip }]
+    theorem Command.loop_unrolling {c: Logic} {b: Command}: [Imp| while (‹c›) { ‹b› }] ≈ [Imp| ite (‹c›) { ‹b›; while (‹c›) { ‹b› }} else { skip }]
       | _, _ =>
         have mp
           | .whileTrue _ _ _ h₁ h₂ h₃ => .ifTrue _ _ h₁ (.seq _ _ _ h₂ h₃)
@@ -200,7 +200,7 @@ namespace SoftwareFoundations.ProgrammingLanguageFoundations.Equiv
           | .ifFalse _ _ h₁ (.skip _) => .whileFalse _ h₁
         ⟨mp, mpr⟩
 
-    theorem Command.seq_assoc {c₁ c₂ c₃: Command}: [Imp| (<[c₁]>; <[c₂]>); <[c₃]>] ≈ [Imp| <[c₁]>; (<[c₂]>; <[c₃]>)]
+    theorem Command.seq_assoc {c₁ c₂ c₃: Command}: [Imp| (‹c₁›; ‹c₂›); ‹c₃›] ≈ [Imp| ‹c₁›; (‹c₂›; ‹c₃›)]
       | _, _ =>
         have mp
           | .seq _ _ _ (.seq _ _ _ h₁ h₂) h₃ => .seq _ _ _ h₁ (.seq _ _ _ h₂ h₃)
@@ -208,7 +208,7 @@ namespace SoftwareFoundations.ProgrammingLanguageFoundations.Equiv
           | .seq _ _ _ h₁ (.seq _ _ _ h₂ h₃) => .seq _ _ _ (.seq _ _ _ h₁ h₂) h₃
         ⟨mp, mpr⟩
 
-    theorem Command.identity_assignment {id: String}: [Imp| <[id]> := <[id:id]>] ≈ [Imp| skip]
+    theorem Command.identity_assignment {id: String}: [Imp| ‹id› := ‹id:id›] ≈ [Imp| skip]
       | _, _ =>
         -- Should use Maps.TotalMap.updateSame
         have mp
@@ -217,7 +217,7 @@ namespace SoftwareFoundations.ProgrammingLanguageFoundations.Equiv
           | .skip _ => sorry
         ⟨mp, mpr⟩
 
-    theorem Command.assign_arith_equiv {id: String} {e: Arith} (h: [Arith| <[id:id]>] ≈ e): [Imp| skip] ≈ [Imp| <[id]> := <[e]> ]
+    theorem Command.assign_arith_equiv {id: String} {e: Arith} (h: [Arith| ‹id:id›] ≈ e): [Imp| skip] ≈ [Imp| ‹id› := ‹e› ]
       | _, _ =>
         have mp
           | .skip _ => sorry
@@ -228,7 +228,7 @@ namespace SoftwareFoundations.ProgrammingLanguageFoundations.Equiv
 
   namespace Tactic
     @[scoped simp]
-    theorem Command.skip_left {c: Command}: [Imp| skip; <[c]>] ≈ c := by
+    theorem Command.skip_left {c: Command}: [Imp| skip; ‹c›] ≈ c := by
       intro s₁ s₂
       apply Iff.intro
       · intro
@@ -251,7 +251,7 @@ namespace SoftwareFoundations.ProgrammingLanguageFoundations.Equiv
             repeat assumption
 
     @[scoped simp]
-    theorem Command.skip_right {c: Command}: [Imp| <[c]>; skip] ≈ c := by
+    theorem Command.skip_right {c: Command}: [Imp| ‹c›; skip] ≈ c := by
       intro s₁ s₂
       apply Iff.intro
       · intro
@@ -273,7 +273,7 @@ namespace SoftwareFoundations.ProgrammingLanguageFoundations.Equiv
             repeat assumption
           · apply CommandEval.skip
 
-    example {t f: Command}: [Imp| ite (tru) { <[t]> } else { <[f]> }] ≈ t := by
+    example {t f: Command}: [Imp| ite (tru) { ‹t› } else { ‹f› }] ≈ t := by
       intro s₁ s₂
       apply Iff.intro
       · intro
@@ -298,7 +298,7 @@ namespace SoftwareFoundations.ProgrammingLanguageFoundations.Equiv
             repeat assumption
 
     @[scoped simp]
-    theorem Command.if_true {b: Logic} {c₁ c₂: Command} (h: b ≈ .true): [Imp| ite (<[b]>) { <[ c₁ ]> } else { <[ c₂ ]> }] ≈ c₁ := by
+    theorem Command.if_true {b: Logic} {c₁ c₂: Command} (h: b ≈ .true): [Imp| ite (‹b›) { ‹c₁› } else { ‹c₂› }] ≈ c₁ := by
       intro s₁ s₂
       apply Iff.intro
       · intro
@@ -324,7 +324,7 @@ namespace SoftwareFoundations.ProgrammingLanguageFoundations.Equiv
             repeat assumption
 
     @[scoped simp]
-    theorem Command.if_false {b: Logic} {c₁ c₂: Command} (h: b ≈ .false): [Imp| ite (<[b]>) { <[ c₁ ]> } else { <[ c₂ ]> }] ≈ c₂ := by
+    theorem Command.if_false {b: Logic} {c₁ c₂: Command} (h: b ≈ .false): [Imp| ite (‹b›) { ‹c₁› } else { ‹c₂› }] ≈ c₂ := by
       intro s₁ s₂
       apply Iff.intro
       · intro
@@ -349,14 +349,14 @@ namespace SoftwareFoundations.ProgrammingLanguageFoundations.Equiv
             . apply CommandEval.whileFalse
               repeat assumption
 
-    theorem Command.if_swap {b: Logic} {c₁ c₂: Command}: [Imp| ite (<[b]>) { <[ c₁ ]> } else { <[ c₂ ]> }] ≈ [Imp| ite (!<[b]>) { <[ c₂ ]> } else { <[ c₁ ]> }] := by
+    theorem Command.if_swap {b: Logic} {c₁ c₂: Command}: [Imp| ite (‹b›) { ‹c₁› } else { ‹c₂› }] ≈ [Imp| ite (!‹b›) { ‹c₂› } else { ‹c₁› }] := by
       intro s₁ s₂
       apply Iff.intro
       · sorry
       · sorry
 
     @[scoped simp]
-    theorem Command.while_false {c: Logic} {b: Command} (h: c ≈ .false): [Imp| while (<[c]>) { <[b]> }] ≈ [Imp| skip] := by
+    theorem Command.while_false {c: Logic} {b: Command} (h: c ≈ .false): [Imp| while (‹c›) { ‹b› }] ≈ [Imp| skip] := by
       intro s₁ s₂
       apply Iff.intro
       · intro
@@ -370,7 +370,7 @@ namespace SoftwareFoundations.ProgrammingLanguageFoundations.Equiv
             · rw [h s₁]
 
     @[scoped simp]
-    theorem Command.while_true {c: Logic} {b: Command} (h: c ≈ .true): [Imp| while (<[c]>) { <[b]> }] ≈ [Imp| while (tru) { skip }] := by
+    theorem Command.while_true {c: Logic} {b: Command} (h: c ≈ .true): [Imp| while (‹c›) { ‹b› }] ≈ [Imp| while (tru) { skip }] := by
       intro s₁ s₂
       apply Iff.intro
       · intro
@@ -391,7 +391,7 @@ namespace SoftwareFoundations.ProgrammingLanguageFoundations.Equiv
           contradiction
         | whileFalse _ _ => simp_all
       where
-        nonterm {c: Logic} {b: Command} {s₁ s₂: State} (h: c ≈ .true): ¬(s₁ =[[Imp| while (<[c]>) { <[b]> }]]=> s₂) := by
+        nonterm {c: Logic} {b: Command} {s₁ s₂: State} (h: c ≈ .true): ¬(s₁ =[[Imp| while (‹c›) { ‹b› }]]=> s₂) := by
           intro
           | .whileTrue s₃ s₄ s₅ h₁ h₂ h₃ =>
             -- simp_all
@@ -399,7 +399,7 @@ namespace SoftwareFoundations.ProgrammingLanguageFoundations.Equiv
             sorry
           | .whileFalse _ _ => simp_all
 
-    theorem Command.loop_unrolling {c: Logic} {b: Command}: [Imp| while (<[ c]>) { <[b]> }] ≈ [Imp| ite (<[c]>) { <[b]>; while (<[c]>) { <[b]> }} else { skip }] := by
+    theorem Command.loop_unrolling {c: Logic} {b: Command}: [Imp| while (‹c›) { ‹b› }] ≈ [Imp| ite (‹c›) { ‹b›; while (‹c›) { ‹b› }} else { skip }] := by
       intro s₁ s₂
       apply Iff.intro
       · intro
@@ -418,7 +418,7 @@ namespace SoftwareFoundations.ProgrammingLanguageFoundations.Equiv
         | .ifFalse _ _ h₁ (.skip _) =>
           exact CommandEval.whileFalse _ h₁
 
-    theorem Command.seq_assoc {c₁ c₂ c₂: Command}: [Imp| (<[c₁]>; <[c₂]>); <[c₃]>] ≈ [Imp| <[c₁]>; (<[c₂]>; <[c₃]>)] := by
+    theorem Command.seq_assoc {c₁ c₂ c₂: Command}: [Imp| (‹c₁›; ‹c₂›); ‹c₃›] ≈ [Imp| ‹c₁›; (‹c₂›; ‹c₃›)] := by
       intro s₁ s₂
       apply Iff.intro
       · intro
@@ -435,13 +435,13 @@ namespace SoftwareFoundations.ProgrammingLanguageFoundations.Equiv
                  repeat assumption)
 
     @[scoped simp]
-    theorem Command.identity_assignment {id: String}: [Imp| <[id]> := <[id:id]>] ≈ [Imp| skip] := by
+    theorem Command.identity_assignment {id: String}: [Imp| ‹id› := ‹id:id›] ≈ [Imp| skip] := by
       intro s₁ s₂
       apply Iff.intro
       · sorry
       · sorry
 
-    theorem Command.assign_arith_equiv {id: String} {e: Arith} (h: [Arith| <[id:id]>] ≈ e): [Imp| skip] ≈ [Imp| <[id]> := <[e]> ] := by
+    theorem Command.assign_arith_equiv {id: String} {e: Arith} (h: [Arith| ‹id:id›] ≈ e): [Imp| skip] ≈ [Imp| ‹id› := ‹e› ] := by
       unfold Command.equiv
       intro s₁ s₂
       apply Iff.intro
@@ -451,7 +451,7 @@ namespace SoftwareFoundations.ProgrammingLanguageFoundations.Equiv
 
   namespace Blended
     @[scoped simp]
-    theorem Command.skip_left {c: Command}: [Imp| skip; <[c]>] ≈ c
+    theorem Command.skip_left {c: Command}: [Imp| skip; ‹c›] ≈ c
       | _, _ =>
         have mp
           | .seq _ _ _ (.skip _) h₂ => h₂
@@ -466,7 +466,7 @@ namespace SoftwareFoundations.ProgrammingLanguageFoundations.Equiv
         ⟨mp, mpr⟩
 
     @[scoped simp]
-    theorem Command.skip_right {c: Command}: [Imp| <[c]>; skip] ≈ c
+    theorem Command.skip_right {c: Command}: [Imp| ‹c›; skip] ≈ c
       | _, _ =>
         have mp
           | .seq _ _ _ h₁ (.skip _) => h₁
@@ -481,7 +481,7 @@ namespace SoftwareFoundations.ProgrammingLanguageFoundations.Equiv
         ⟨mp, mpr⟩
 
     @[scoped simp]
-    example {t f: Command}: [Imp| ite (tru) { <[t]> } else { <[f]> }] ≈ t
+    example {t f: Command}: [Imp| ite (tru) { ‹t› } else { ‹f› }] ≈ t
       | _, _ =>
         have mp
           | .ifTrue _ _ _ h₂ => h₂
@@ -497,7 +497,7 @@ namespace SoftwareFoundations.ProgrammingLanguageFoundations.Equiv
         ⟨mp, mpr⟩
 
     @[scoped simp]
-    theorem Command.if_true {b: Logic} {c₁ c₂: Command} (h: b ≈ .true): [Imp| ite (<[b]>) { <[ c₁ ]> } else { <[ c₂ ]> }] ≈ c₁
+    theorem Command.if_true {b: Logic} {c₁ c₂: Command} (h: b ≈ .true): [Imp| ite (‹b›) { ‹c₁› } else { ‹c₂› }] ≈ c₁
       | _, _ =>
         have truu: b.eval _ = Logic.true.eval _ := h _
         have mp
@@ -514,7 +514,7 @@ namespace SoftwareFoundations.ProgrammingLanguageFoundations.Equiv
         ⟨mp, mpr⟩
 
     @[scoped simp]
-    theorem Command.if_false {b: Logic} {c₁ c₂: Command} (h: b ≈ .false): [Imp| ite (<[b]>) { <[ c₁ ]> } else { <[ c₂ ]> }] ≈ c₂
+    theorem Command.if_false {b: Logic} {c₁ c₂: Command} (h: b ≈ .false): [Imp| ite (‹b›) { ‹c₁› } else { ‹c₂› }] ≈ c₂
       | _, _ =>
         have falz: b.eval _ = Logic.false.eval _ := h _
         have mp
@@ -530,10 +530,10 @@ namespace SoftwareFoundations.ProgrammingLanguageFoundations.Equiv
           | .whileFalse _ h₁          => .ifFalse _ _ falz (.whileFalse _ h₁)
         ⟨mp, mpr⟩
 
-    theorem Command.if_swap {b: Logic} {c₁ c₂: Command}: [Imp| ite (<[b]>) { <[ c₁ ]> } else { <[ c₂ ]> }] ≈ [Imp| ite (!<[b]>) { <[ c₂ ]> } else { <[ c₁ ]> }] := sorry
+    theorem Command.if_swap {b: Logic} {c₁ c₂: Command}: [Imp| ite (‹b›) { ‹c₁› } else { ‹c₂› }] ≈ [Imp| ite (!‹b›) { ‹c₂› } else { ‹c₁› }] := sorry
 
     @[scoped simp]
-    theorem Command.while_false {c: Logic} {b: Command} (h: c ≈ .false): [Imp| while (<[c]>) { <[b]> }] ≈ [Imp| skip]
+    theorem Command.while_false {c: Logic} {b: Command} (h: c ≈ .false): [Imp| while (‹c›) { ‹b› }] ≈ [Imp| skip]
       | _, _ =>
         have falz: c.eval _ = Logic.false.eval _ := h _
         have mp
@@ -544,7 +544,7 @@ namespace SoftwareFoundations.ProgrammingLanguageFoundations.Equiv
         ⟨mp, mpr⟩
 
     @[scoped simp]
-    theorem Command.while_true {c: Logic} {b: Command} (h: c ≈ .true): [Imp| while (<[c]>) { <[b]> }] ≈ [Imp| while (tru) { skip }]
+    theorem Command.while_true {c: Logic} {b: Command} (h: c ≈ .true): [Imp| while (‹c›) { ‹b› }] ≈ [Imp| while (tru) { skip }]
       | _, _ =>
         have truu: c.eval _ = Logic.true.eval _ := h _
         have hh: Logic.true.equiv .true
@@ -557,11 +557,11 @@ namespace SoftwareFoundations.ProgrammingLanguageFoundations.Equiv
           | .whileFalse _ h₁ => Logic.true.trueFalse rfl h₁
         ⟨mp, mpr⟩
       where
-        nonterm {c: Logic} {b: Command} {s₁ s₂: State} (h: c ≈ .true): ¬(s₁ =[[Imp| while (<[c]>) { <[b]> }]]=> s₂)
+        nonterm {c: Logic} {b: Command} {s₁ s₂: State} (h: c ≈ .true): ¬(s₁ =[[Imp| while (‹c›) { ‹b› }]]=> s₂)
           | .whileTrue _ _ _ _ _ h₃ => sorry
           | .whileFalse _ h₁ => c.trueFalse (h _) h₁
 
-    theorem Command.loop_unrolling {c: Logic} {b: Command}: [Imp| while (<[c]>) { <[b]> }] ≈ [Imp| ite (<[c]>) { <[b]>; while (<[c]>) { <[b]> }} else { skip }]
+    theorem Command.loop_unrolling {c: Logic} {b: Command}: [Imp| while (‹c›) { ‹b› }] ≈ [Imp| ite (‹c›) { ‹b›; while (‹c›) { ‹b› }} else { skip }]
       | _, _ =>
         have mp
           | .whileTrue _ _ _ h₁ h₂ h₃ => .ifTrue _ _ h₁ (.seq _ _ _ h₂ h₃)
@@ -571,7 +571,7 @@ namespace SoftwareFoundations.ProgrammingLanguageFoundations.Equiv
           | .ifFalse _ _ h₁ (.skip _) => .whileFalse _ h₁
         ⟨mp, mpr⟩
 
-    theorem Command.seq_assoc {c₁ c₂ c₃: Command}: [Imp| (<[c₁]>; <[c₂]>); <[c₃]>] ≈ [Imp| <[c₁]>; (<[c₂]>; <[c₃]>)]
+    theorem Command.seq_assoc {c₁ c₂ c₃: Command}: [Imp| (‹c₁›; ‹c₂›); ‹c₃›] ≈ [Imp| ‹c₁›; (‹c₂›; ‹c₃›)]
       | _, _ =>
         have mp
           | .seq _ _ _ (.seq _ _ _ h₁ h₂) h₃ => .seq _ _ _ h₁ (.seq _ _ _ h₂ h₃)
@@ -580,9 +580,9 @@ namespace SoftwareFoundations.ProgrammingLanguageFoundations.Equiv
         ⟨mp, mpr⟩
 
     @[scoped simp]
-    theorem Command.identity_assignment {id: String}: [Imp| <[id]> := <[id:id]>] ≈ [Imp| skip] := by sorry
+    theorem Command.identity_assignment {id: String}: [Imp| ‹id› := ‹id:id›] ≈ [Imp| skip] := by sorry
 
-    theorem Command.assign_arith_equiv {id: String} {e: Arith} (h: [Arith| <[id:id]>] ≈ e): [Imp| skip] ≈ [Imp| <[id]> := <[e]> ] := by sorry
+    theorem Command.assign_arith_equiv {id: String} {e: Arith} (h: [Arith| ‹id:id›] ≈ e): [Imp| skip] ≈ [Imp| ‹id› := ‹e› ] := by sorry
   end Blended
 
   section
@@ -818,9 +818,9 @@ namespace SoftwareFoundations.ProgrammingLanguageFoundations.Equiv
     theorem Command.skip.congr: [Imp| skip] ≈ [Imp| skip]
       | _, _ => Iff.refl _
 
-    theorem Command.assign.congr {id: String} {e₁ e₂: Arith} (h₁: e₁ ≈ e₂): [Imp| <[id]> := <[e₁]> ].equiv [Imp| <[id]> := <[e₂]>]
+    theorem Command.assign.congr {id: String} {e₁ e₂: Arith} (h₁: e₁ ≈ e₂): [Imp| ‹id› := ‹e₁› ].equiv [Imp| ‹id› := ‹e₂›]
       | s₁, s₂ =>
-        have h {id: String} {e₁ e₂: Arith} (h: e₁ ≈ e₂): (s₁ =[[Imp| <[id]> := <[e₁]>]]=> s₂) → s₁ =[[Imp| <[id]> := <[e₂]>]]=> s₂
+        have h {id: String} {e₁ e₂: Arith} (h: e₁ ≈ e₂): (s₁ =[[Imp| ‹id› := ‹e₁›]]=> s₂) → s₁ =[[Imp| ‹id› := ‹e₂›]]=> s₂
           | .assign _ h₁ =>
             have h₂: e₂.eval _ = _ :=
               calc e₂.eval _
@@ -830,9 +830,9 @@ namespace SoftwareFoundations.ProgrammingLanguageFoundations.Equiv
         have h₂ := Arith.equiv.symm h₁
         ⟨h h₁, h h₂⟩
 
-    theorem Command.seq.congr {c₁ c₂ c₃ c₄: Command} (h₁: c₁ ≈ c₂) (h₂: c₃ ≈ c₄): [Imp| <[c₁]>; <[c₃]>] ≈ [Imp| <[c₂]>; <[c₄]>]
+    theorem Command.seq.congr {c₁ c₂ c₃ c₄: Command} (h₁: c₁ ≈ c₂) (h₂: c₃ ≈ c₄): [Imp| ‹c₁›; ‹c₃›] ≈ [Imp| ‹c₂›; ‹c₄›]
       | s₁, s₂ =>
-        have h {c₁ c₂ c₃ c₄: Command} (h₁: c₁ ≈ c₂) (h₂: c₃ ≈ c₄): (s₁ =[[Imp| <[c₁]>; <[c₃]>]]=> s₂) → s₁ =[[Imp| <[c₂]>; <[c₄]>]]=> s₂
+        have h {c₁ c₂ c₃ c₄: Command} (h₁: c₁ ≈ c₂) (h₂: c₃ ≈ c₄): (s₁ =[[Imp| ‹c₁›; ‹c₃›]]=> s₂) → s₁ =[[Imp| ‹c₂›; ‹c₄›]]=> s₂
           | .seq _ _ _ h₃ h₄ =>
             have h₅: _ =[c₂]=> _ :=
               have ⟨h, _⟩ := h₁ _ _
@@ -845,9 +845,9 @@ namespace SoftwareFoundations.ProgrammingLanguageFoundations.Equiv
         have h₄ := Command.equiv.symm h₂
         ⟨h h₁ h₂, h h₃ h₄⟩
 
-    theorem Command.if.congr {c₁ c₂: Logic} {t₁ t₂ f₁ f₂: Command} (h₁: c₁ ≈ c₂) (h₂: t₁ ≈ t₂) (h₃: f₁ ≈ f₂): [Imp| ite (<[c₁]>) { <[t₁]> } else { <[f₁]> }] ≈ [Imp| ite (<[c₂]>) { <[t₂]> } else { <[f₂]> }]
+    theorem Command.if.congr {c₁ c₂: Logic} {t₁ t₂ f₁ f₂: Command} (h₁: c₁ ≈ c₂) (h₂: t₁ ≈ t₂) (h₃: f₁ ≈ f₂): [Imp| ite (‹c₁›) { ‹t₁› } else { ‹f₁› }] ≈ [Imp| ite (‹c₂›) { ‹t₂› } else { ‹f₂› }]
       | s₁, s₂ =>
-        have h {c₁ c₂: Logic} {t₁ t₂ f₁ f₂: Command} (h₁: c₁ ≈ c₂) (h₂: t₁ ≈ t₂) (h₃: f₁ ≈ f₂): (s₁ =[[Imp| ite (<[c₁]>) { <[t₁]> } else { <[f₁]> }]]=> s₂) → s₁ =[[Imp| ite (<[c₂]>) { <[t₂]> } else { <[f₂]> }]]=> s₂
+        have h {c₁ c₂: Logic} {t₁ t₂ f₁ f₂: Command} (h₁: c₁ ≈ c₂) (h₂: t₁ ≈ t₂) (h₃: f₁ ≈ f₂): (s₁ =[[Imp| ite (‹c₁›) { ‹t₁› } else { ‹f₁› }]]=> s₂) → s₁ =[[Imp| ite (‹c₂›) { ‹t₂› } else { ‹f₂› }]]=> s₂
           | .ifTrue _ _ h₄ h₅ =>
             have h₆: c₂.eval _ = true :=
               calc c₂.eval _
@@ -871,9 +871,9 @@ namespace SoftwareFoundations.ProgrammingLanguageFoundations.Equiv
         have h₆ := Command.equiv.symm h₃
         ⟨h h₁ h₂ h₃, h h₄ h₅ h₆⟩
 
-    theorem Command.while.congr {c₁ c₂: Logic} {b₁ b₂: Command} (h₁: c₁ ≈ c₂) (h₂: b₁ ≈ b₂): [Imp| while (<[c₁]>) { <[b₁]> }] ≈ [Imp| while (<[c₂]>) { <[b₂]> }]
+    theorem Command.while.congr {c₁ c₂: Logic} {b₁ b₂: Command} (h₁: c₁ ≈ c₂) (h₂: b₁ ≈ b₂): [Imp| while (‹c₁›) { ‹b₁› }] ≈ [Imp| while (‹c₂›) { ‹b₂› }]
       | s₁, s₂ =>
-        have h {c₁ c₂: Logic} {b₁ b₂: Command} (h₁: c₁ ≈ c₂) (h₂: b₁ ≈ b₂): (s₁ =[[Imp| while (<[c₁]>) { <[b₁]> }]]=> s₂) → s₁ =[[Imp| while (<[c₂]>) { <[b₂]> }]]=> s₂
+        have h {c₁ c₂: Logic} {b₁ b₂: Command} (h₁: c₁ ≈ c₂) (h₂: b₁ ≈ b₂): (s₁ =[[Imp| while (‹c₁›) { ‹b₁› }]]=> s₂) → s₁ =[[Imp| while (‹c₂›) { ‹b₂› }]]=> s₂
           | .whileTrue _ _ _ h₄ h₅ h₆ =>
             have h₇: c₂.eval _ = true :=
               calc c₂.eval _
@@ -882,7 +882,7 @@ namespace SoftwareFoundations.ProgrammingLanguageFoundations.Equiv
             have h₈: _ =[b₂]=> _ :=
               have ⟨h, _⟩ := h₂ _ _
               h h₅
-            have h₉: _ =[[Imp| while (<[c₂]>) { <[b₂]> }]]=> _ :=
+            have h₉: _ =[[Imp| while (‹c₂›) { ‹b₂› }]]=> _ :=
               -- have h₁ := h₁ _
               -- have ⟨h₁, _⟩ := h₂ _ _
               -- h₆ h₁ h₂
@@ -914,9 +914,9 @@ namespace SoftwareFoundations.ProgrammingLanguageFoundations.Equiv
       intro s₁ s₂
       apply Iff.refl
 
-    theorem Command.assign.congr {id: String} {e₁ e₂: Arith} (h₁: e₁ ≈ e₂): [Imp| <[id]> := <[e₁]> ].equiv [Imp| <[id]> := <[e₂]>] := by
+    theorem Command.assign.congr {id: String} {e₁ e₂: Arith} (h₁: e₁ ≈ e₂): [Imp| ‹id› := ‹e₁› ].equiv [Imp| ‹id› := ‹e₂›] := by
       intro s₁ s₂
-      have h {id: String} {e₁ e₂: Arith} (h₁: e₁ ≈ e₂): (s₁ =[[Imp| <[id]> := <[e₁]>]]=> s₂) → s₁ =[[Imp| <[id]> := <[e₂]>]]=> s₂ := by
+      have h {id: String} {e₁ e₂: Arith} (h₁: e₁ ≈ e₂): (s₁ =[[Imp| ‹id› := ‹e₁›]]=> s₂) → s₁ =[[Imp| ‹id› := ‹e₂›]]=> s₂ := by
         intro
         | .assign _ h =>
           rw [h₁] at h
@@ -926,9 +926,9 @@ namespace SoftwareFoundations.ProgrammingLanguageFoundations.Equiv
       · apply h
         · exact Arith.equiv.symm h₁
 
-    theorem Command.seq.congr {c₁ c₂ c₃ c₄: Command} (h₁: c₁ ≈ c₂) (h₂: c₃ ≈ c₄): [Imp| <[c₁]>; <[c₃]>] ≈ [Imp| <[c₂]>; <[c₄]>] := by
+    theorem Command.seq.congr {c₁ c₂ c₃ c₄: Command} (h₁: c₁ ≈ c₂) (h₂: c₃ ≈ c₄): [Imp| ‹c₁›; ‹c₃›] ≈ [Imp| ‹c₂›; ‹c₄›] := by
       intro s₁ s₂
-      have h {c₁ c₂ c₃ c₄: Command} (h₁: c₁ ≈ c₂) (h₂: c₃ ≈ c₄): (s₁ =[[Imp| <[c₁]>; <[c₃]>]]=> s₂) → s₁ =[[Imp| <[c₂]>; <[c₄]>]]=> s₂ := by
+      have h {c₁ c₂ c₃ c₄: Command} (h₁: c₁ ≈ c₂) (h₂: c₃ ≈ c₄): (s₁ =[[Imp| ‹c₁›; ‹c₃›]]=> s₂) → s₁ =[[Imp| ‹c₂›; ‹c₄›]]=> s₂ := by
         intro
         | .seq _ _ _ h₃ h₄ =>
           rw [h₁] at h₃
@@ -940,9 +940,9 @@ namespace SoftwareFoundations.ProgrammingLanguageFoundations.Equiv
         · exact Command.equiv.symm h₁
         · exact Command.equiv.symm h₂
 
-    theorem Command.if.congr {c₁ c₂: Logic} {t₁ t₂ f₁ f₂: Command} (h₁: c₁ ≈ c₂) (h₂: t₁ ≈ t₂) (h₃: f₁ ≈ f₂): [Imp| ite (<[c₁]>) { <[t₁]> } else { <[f₁]> }] ≈ [Imp| ite (<[c₂]>) { <[t₂]> } else { <[f₂]> }] := by
+    theorem Command.if.congr {c₁ c₂: Logic} {t₁ t₂ f₁ f₂: Command} (h₁: c₁ ≈ c₂) (h₂: t₁ ≈ t₂) (h₃: f₁ ≈ f₂): [Imp| ite (‹c₁›) { ‹t₁› } else { ‹f₁› }] ≈ [Imp| ite (‹c₂›) { ‹t₂› } else { ‹f₂› }] := by
       intro s₁ s₂
-      have h {c₁ c₂: Logic} {t₁ t₂ f₁ f₂: Command} (h₁: c₁ ≈ c₂) (h₂: t₁ ≈ t₂) (h₃: f₁ ≈ f₂): (s₁ =[[Imp| ite (<[c₁]>) { <[t₁]> } else { <[f₁]> }]]=> s₂) → s₁ =[[Imp| ite (<[c₂]>) { <[t₂]> } else { <[f₂]> }]]=> s₂ := by
+      have h {c₁ c₂: Logic} {t₁ t₂ f₁ f₂: Command} (h₁: c₁ ≈ c₂) (h₂: t₁ ≈ t₂) (h₃: f₁ ≈ f₂): (s₁ =[[Imp| ite (‹c₁›) { ‹t₁› } else { ‹f₁› }]]=> s₂) → s₁ =[[Imp| ite (‹c₂›) { ‹t₂› } else { ‹f₂› }]]=> s₂ := by
         intro
         | .ifTrue _ _ h₄ h₅ =>
           rw [h₁] at h₄
@@ -959,14 +959,14 @@ namespace SoftwareFoundations.ProgrammingLanguageFoundations.Equiv
         · exact Command.equiv.symm h₂
         · exact Command.equiv.symm h₃
 
-    theorem Command.while.congr {c₁ c₂: Logic} {b₁ b₂: Command} (h₁: c₁ ≈ c₂) (h₂: b₁ ≈ b₂): [Imp| while (<[c₁]>) { <[b₁]> }] ≈ [Imp| while (<[c₂]>) { <[b₂]> }] := by
+    theorem Command.while.congr {c₁ c₂: Logic} {b₁ b₂: Command} (h₁: c₁ ≈ c₂) (h₂: b₁ ≈ b₂): [Imp| while (‹c₁›) { ‹b₁› }] ≈ [Imp| while (‹c₂›) { ‹b₂› }] := by
       intro s₁ s₂
-      have h {c₁ c₂: Logic} {b₁ b₂: Command} (h₁: c₁ ≈ c₂) (h₂: b₁ ≈ b₂): (s₁ =[[Imp| while (<[c₁]>) { <[b₁]> }]]=> s₂) → s₁ =[[Imp| while (<[c₂]>) { <[b₂]> }]]=> s₂ := by
+      have h {c₁ c₂: Logic} {b₁ b₂: Command} (h₁: c₁ ≈ c₂) (h₂: b₁ ≈ b₂): (s₁ =[[Imp| while (‹c₁›) { ‹b₁› }]]=> s₂) → s₁ =[[Imp| while (‹c₂›) { ‹b₂› }]]=> s₂ := by
         intro
         | .whileTrue s₃ s₄ s₅ h₃ h₄ h₅ =>
           rw [h₁] at h₃
           rw [h₂] at h₄
-          have ih: s₄ =[[Imp| while (<[c₂]>) { <[ b₂ ]>}]]=> s₅ := by
+          have ih: s₄ =[[Imp| while (‹c₂›) { ‹b₂›}]]=> s₅ := by
             sorry
           exact CommandEval.whileTrue _ _ _ h₃ h₄ ih
         | .whileFalse _ h₃ =>
@@ -985,18 +985,18 @@ namespace SoftwareFoundations.ProgrammingLanguageFoundations.Equiv
     theorem Command.skip.congr: [Imp| skip] ≈ [Imp| skip]
       | _, _ => Iff.refl _
 
-    theorem Command.assign.congr {id: String} {e₁ e₂: Arith} (h₁: e₁ ≈ e₂): [Imp| <[id]> := <[e₁]> ].equiv [Imp| <[id]> := <[e₂]>]
+    theorem Command.assign.congr {id: String} {e₁ e₂: Arith} (h₁: e₁ ≈ e₂): [Imp| ‹id› := ‹e₁› ].equiv [Imp| ‹id› := ‹e₂›]
       | s₁, s₂ =>
-        have h {id: String} {e₁ e₂: Arith} (h₁: e₁ ≈ e₂): (s₁ =[[Imp| <[id]> := <[e₁]>]]=> s₂) → s₁ =[[Imp| <[id]> := <[e₂]>]]=> s₂
+        have h {id: String} {e₁ e₂: Arith} (h₁: e₁ ≈ e₂): (s₁ =[[Imp| ‹id› := ‹e₁›]]=> s₂) → s₁ =[[Imp| ‹id› := ‹e₂›]]=> s₂
           | .assign _ h => by
             rw [h₁] at h
             exact CommandEval.assign _ h
         have h₂ := Arith.equiv.symm h₁
         ⟨h h₁, h h₂⟩
 
-    theorem Command.seq.congr {c₁ c₂ c₃ c₄: Command} (h₁: c₁ ≈ c₂) (h₂: c₃ ≈ c₄): [Imp| <[c₁]>; <[c₃]>] ≈ [Imp| <[c₂]>; <[c₄]>]
+    theorem Command.seq.congr {c₁ c₂ c₃ c₄: Command} (h₁: c₁ ≈ c₂) (h₂: c₃ ≈ c₄): [Imp| ‹c₁›; ‹c₃›] ≈ [Imp| ‹c₂›; ‹c₄›]
       | s₁, s₂ =>
-        have h {c₁ c₂ c₃ c₄: Command} (h₁: c₁ ≈ c₂) (h₂: c₃ ≈ c₄): (s₁ =[[Imp| <[c₁]>; <[c₃]>]]=> s₂) → s₁ =[[Imp| <[c₂]>; <[c₄]>]]=> s₂
+        have h {c₁ c₂ c₃ c₄: Command} (h₁: c₁ ≈ c₂) (h₂: c₃ ≈ c₄): (s₁ =[[Imp| ‹c₁›; ‹c₃›]]=> s₂) → s₁ =[[Imp| ‹c₂›; ‹c₄›]]=> s₂
           | .seq _ _ _ h₃ h₄ => by
             rw [h₁] at h₃
             rw [h₂] at h₄
@@ -1005,9 +1005,9 @@ namespace SoftwareFoundations.ProgrammingLanguageFoundations.Equiv
         have h₄ := Command.equiv.symm h₂
         ⟨h h₁ h₂, h h₃ h₄⟩
 
-    theorem Command.if.congr {c₁ c₂: Logic} {t₁ t₂ f₁ f₂: Command} (h₁: c₁ ≈ c₂) (h₂: t₁ ≈ t₂) (h₃: f₁ ≈ f₂): [Imp| ite (<[c₁]>) { <[t₁]> } else { <[f₁]> }] ≈ [Imp| ite (<[c₂]>) { <[t₂]> } else { <[f₂]> }]
+    theorem Command.if.congr {c₁ c₂: Logic} {t₁ t₂ f₁ f₂: Command} (h₁: c₁ ≈ c₂) (h₂: t₁ ≈ t₂) (h₃: f₁ ≈ f₂): [Imp| ite (‹c₁›) { ‹t₁› } else { ‹f₁› }] ≈ [Imp| ite (‹c₂›) { ‹t₂› } else { ‹f₂› }]
       | s₁, s₂ =>
-        have h {c₁ c₂: Logic} {t₁ t₂ f₁ f₂: Command} (h₁: c₁ ≈ c₂) (h₂: t₁ ≈ t₂) (h₃: f₁ ≈ f₂): (s₁ =[[Imp| ite (<[c₁]>) { <[t₁]> } else { <[f₁]> }]]=> s₂) → s₁ =[[Imp| ite (<[c₂]>) { <[t₂]> } else { <[f₂]> }]]=> s₂
+        have h {c₁ c₂: Logic} {t₁ t₂ f₁ f₂: Command} (h₁: c₁ ≈ c₂) (h₂: t₁ ≈ t₂) (h₃: f₁ ≈ f₂): (s₁ =[[Imp| ite (‹c₁›) { ‹t₁› } else { ‹f₁› }]]=> s₂) → s₁ =[[Imp| ite (‹c₂›) { ‹t₂› } else { ‹f₂› }]]=> s₂
           | .ifTrue _ _ h₄ h₅ => by
             rw [h₁] at h₄
             rw [h₂] at h₅
@@ -1021,9 +1021,9 @@ namespace SoftwareFoundations.ProgrammingLanguageFoundations.Equiv
         have h₆ := Command.equiv.symm h₃
         ⟨h h₁ h₂ h₃, h h₄ h₅ h₆⟩
 
-    theorem Command.while.congr {c₁ c₂: Logic} {b₁ b₂: Command} (h₁: c₁ ≈ c₂) (h₂: b₁ ≈ b₂): [Imp| while (<[c₁]>) { <[b₁]> }] ≈ [Imp| while (<[c₂]>) { <[b₂]> }]
+    theorem Command.while.congr {c₁ c₂: Logic} {b₁ b₂: Command} (h₁: c₁ ≈ c₂) (h₂: b₁ ≈ b₂): [Imp| while (‹c₁›) { ‹b₁› }] ≈ [Imp| while (‹c₂›) { ‹b₂› }]
       | s₁, s₂ =>
-        have h {c₁ c₂: Logic} {b₁ b₂: Command} (h₁: c₁ ≈ c₂) (h₂: b₁ ≈ b₂): (s₁ =[[Imp| while (<[c₁]>) { <[b₁]> }]]=> s₂) → s₁ =[[Imp| while (<[c₂]>) { <[b₂]> }]]=> s₂
+        have h {c₁ c₂: Logic} {b₁ b₂: Command} (h₁: c₁ ≈ c₂) (h₂: b₁ ≈ b₂): (s₁ =[[Imp| while (‹c₁›) { ‹b₁› }]]=> s₂) → s₁ =[[Imp| while (‹c₂›) { ‹b₂› }]]=> s₂
           | .whileTrue s₃ s₄ s₅ h₃ h₄ h₅ => by
             rw [h₁] at h₃
             rw [h₂] at h₄
@@ -1194,21 +1194,21 @@ namespace SoftwareFoundations.ProgrammingLanguageFoundations.Equiv
         have ih₁ := sound e₁ s
         have ih₂ := sound e₂ s
         have h :=
-          calc [Arith| <[e₁]> - <[e₂]>].eval s
+          calc [Arith| ‹e₁› - ‹e₂›].eval s
             _ = e₁.eval s - e₂.eval s                                         := rfl
             _ = e₁.constFold.eval s - e₂.constFold.eval s                     := congr (congrArg Nat.sub ih₁) ih₂
-            _ = [Arith| <[e₁.constFold]> - <[e₂.constFold]>].eval s := rfl
-            -- _ = [Arith| <[e₁]> - <[e₂]>].eval s                     := sorry
+            _ = [Arith| ‹e₁.constFold› - ‹e₂.constFold›].eval s := rfl
+            -- _ = [Arith| ‹e₁› - ‹e₂›].eval s                     := sorry
         sorry
       | .mult e₁ e₂, s =>
         have ih₁ := sound e₁ s
         have ih₂ := sound e₂ s
         have h :=
-          calc [Arith| <[e₁]> * <[e₂]>].eval s
+          calc [Arith| ‹e₁› * ‹e₂›].eval s
             _ = e₁.eval s * e₂.eval s                                         := rfl
             _ = e₁.constFold.eval s * e₂.constFold.eval s                     := congr (congrArg Nat.mul ih₁) ih₂
-            _ = [Arith| <[e₁.constFold]> * <[e₂.constFold]>].eval s := rfl
-            -- _ = [Arith| <[e₁]> * <[e₂]>].eval s                     := sorry
+            _ = [Arith| ‹e₁.constFold› * ‹e₂.constFold›].eval s := rfl
+            -- _ = [Arith| ‹e₁› * ‹e₂›].eval s                     := sorry
         sorry
 
     theorem Logic.constFold.sound: Logic.transform_sound Logic.constFold := sorry
@@ -1289,97 +1289,97 @@ namespace SoftwareFoundations.ProgrammingLanguageFoundations.Equiv
           | .num n =>
             match n with
               | .zero =>
-                calc [Arith| 0 + <[e₂]>].eval s
+                calc [Arith| 0 + ‹e₂›].eval s
                   _ = [Arith| 0].eval s + e₂.eval s                                       := rfl
                   _ = [Arith| 0].opt0Plus.eval s + e₂.opt0Plus.eval s                     := congr (congrArg Nat.add ih₁) ih₂
-                  _ = [Arith| <[[Arith| 0].opt0Plus]> + <[e₂.opt0Plus]>].eval s := rfl
-                  _ = [Arith| 0 + <[e₂]>].opt0Plus.eval s                            := by simp -- congrArg (Arith.eval s) rfl -- TODO: Remove Tactic Block
+                  _ = [Arith| ‹[Arith| 0].opt0Plus› + ‹e₂.opt0Plus›].eval s := rfl
+                  _ = [Arith| 0 + ‹e₂›].opt0Plus.eval s                            := by simp -- congrArg (Arith.eval s) rfl -- TODO: Remove Tactic Block
                   _ = e₂.opt0Plus.eval s                                                  := rfl
               | .succ _ =>
-                calc [Arith| <[num:Nat.succ _]> + <[e₂]>].eval s
+                calc [Arith| ‹num:Nat.succ _› + ‹e₂›].eval s
                   _ = (Arith.num (.succ _)).eval s + e₂.eval s                   := rfl
                   _ = (Arith.num (.succ _)).opt0Plus.eval s + e₂.opt0Plus.eval s := congr (congrArg Nat.add ih₁) ih₂
                   _ = (Arith.plus (.num (.succ _)) e₂).opt0Plus.eval s           := rfl
           | .ident _ =>
-            calc [Arith| <[id:_]> + <[e₂]>].eval s
-              _ = [Arith| <[id:_]>].eval s + e₂.eval s                   := rfl
-              _ = [Arith| <[id:_]>].opt0Plus.eval s + e₂.opt0Plus.eval s := congr (congrArg Nat.add ih₁) ih₂
-              _ = [Arith| <[id:_]> + <[e₂]>].opt0Plus.eval s        := rfl
+            calc [Arith| ‹id:_› + ‹e₂›].eval s
+              _ = [Arith| ‹id:_›].eval s + e₂.eval s                   := rfl
+              _ = [Arith| ‹id:_›].opt0Plus.eval s + e₂.opt0Plus.eval s := congr (congrArg Nat.add ih₁) ih₂
+              _ = [Arith| ‹id:_› + ‹e₂›].opt0Plus.eval s        := rfl
           | .plus _ _ =>
-            calc [Arith| (<[_]> + <[_]>) + <[e₂]>].eval s
-              _ = [Arith| <[_]> + <[_]>].eval s + e₂.eval s                   := rfl
-              _ = [Arith| <[_]> + <[_]>].opt0Plus.eval s + e₂.opt0Plus.eval s := congr (congrArg Nat.add ih₁) ih₂
-              _ = [Arith| (<[_]> + <[_]>) + <[e₂]>].opt0Plus.eval s      := rfl
+            calc [Arith| (‹_› + ‹_›) + ‹e₂›].eval s
+              _ = [Arith| ‹_› + ‹_›].eval s + e₂.eval s                   := rfl
+              _ = [Arith| ‹_› + ‹_›].opt0Plus.eval s + e₂.opt0Plus.eval s := congr (congrArg Nat.add ih₁) ih₂
+              _ = [Arith| (‹_› + ‹_›) + ‹e₂›].opt0Plus.eval s      := rfl
           | .minus _ _ =>
-            calc [Arith| (<[_]> - <[_]>) + <[e₂]>].eval s
-              _ = [Arith| <[_]> - <[_]>].eval s + e₂.eval s                   := rfl
-              _ = [Arith| <[_]> - <[_]>].opt0Plus.eval s + e₂.opt0Plus.eval s := congr (congrArg Nat.add ih₁) ih₂
-              _ = [Arith| (<[_]> - <[_]>) + <[e₂]>].opt0Plus.eval s      := rfl
+            calc [Arith| (‹_› - ‹_›) + ‹e₂›].eval s
+              _ = [Arith| ‹_› - ‹_›].eval s + e₂.eval s                   := rfl
+              _ = [Arith| ‹_› - ‹_›].opt0Plus.eval s + e₂.opt0Plus.eval s := congr (congrArg Nat.add ih₁) ih₂
+              _ = [Arith| (‹_› - ‹_›) + ‹e₂›].opt0Plus.eval s      := rfl
           | .mult _ _ =>
-            calc [Arith| (<[_]> * <[_]>) + <[e₂]>].eval s
-              _ = [Arith| <[_]> * <[_]>].eval s + e₂.eval s                   := rfl
-              _ = [Arith| <[_]> * <[_]>].opt0Plus.eval s + e₂.opt0Plus.eval s := congr (congrArg Nat.add ih₁) ih₂
-              _ = [Arith| (<[_]> * <[_]>) + <[e₂]>].opt0Plus.eval s      := rfl
+            calc [Arith| (‹_› * ‹_›) + ‹e₂›].eval s
+              _ = [Arith| ‹_› * ‹_›].eval s + e₂.eval s                   := rfl
+              _ = [Arith| ‹_› * ‹_›].opt0Plus.eval s + e₂.opt0Plus.eval s := congr (congrArg Nat.add ih₁) ih₂
+              _ = [Arith| (‹_› * ‹_›) + ‹e₂›].opt0Plus.eval s      := rfl
       | .minus e₁ e₂, s =>
         have ih₁ := sound e₁ s
         have ih₂ := sound e₂ s
-        calc [Arith| <[e₁]> - <[e₂]>].eval s
+        calc [Arith| ‹e₁› - ‹e₂›].eval s
           _ = e₁.eval s - e₂.eval s                              := rfl
           _ = e₁.opt0Plus.eval s - e₂.opt0Plus.eval s            := congr (congrArg Nat.sub ih₁) ih₂
-          _ = [Arith| <[e₁]> - <[e₂]>].opt0Plus.eval s := rfl
+          _ = [Arith| ‹e₁› - ‹e₂›].opt0Plus.eval s := rfl
       | .mult e₁ e₂, s =>
         have ih₁ := sound e₁ s
         have ih₂ := sound e₂ s
-        calc [Arith| <[e₁]> * <[e₂]>].eval s
+        calc [Arith| ‹e₁› * ‹e₂›].eval s
           _ = e₁.eval s * e₂.eval s                              := rfl
           _ = e₁.opt0Plus.eval s * e₂.opt0Plus.eval s            := congr (congrArg Nat.mul ih₁) ih₂
-          _ = [Arith| <[e₁]> * <[e₂]>].opt0Plus.eval s := rfl
+          _ = [Arith| ‹e₁› * ‹e₂›].opt0Plus.eval s := rfl
 
     theorem Logic.opt0Plus.sound: Logic.transform_sound Logic.opt0Plus
       | .true, _ | .false, _ => rfl
       | .eq e₁ e₂, s =>
         have ih₁ := Arith.opt0Plus.sound e₁ s
         have ih₂ := Arith.opt0Plus.sound e₂ s
-        calc [Logic| <[e₁]> = <[e₂]>].eval s
+        calc [Logic| ‹e₁› = ‹e₂›].eval s
           _ = BEq.beq (e₁.eval s) (e₂.eval s)                   := rfl
           _ = BEq.beq (e₁.opt0Plus.eval s) (e₂.opt0Plus.eval s) := congr (congrArg BEq.beq ih₁) ih₂
-          _ = [Logic| <[e₁]> = <[e₂]>].opt0Plus.eval s                  := rfl
+          _ = [Logic| ‹e₁› = ‹e₂›].opt0Plus.eval s                  := rfl
       | .neq e₁ e₂, s =>
         have ih₁ := Arith.opt0Plus.sound e₁ s
         have ih₂ := Arith.opt0Plus.sound e₂ s
-        calc [Logic| <[e₁]> ≠ <[e₂]>].eval s
+        calc [Logic| ‹e₁› ≠ ‹e₂›].eval s
           _ = not (BEq.beq (e₁.eval s) (e₂.eval s))                   := rfl
           _ = not (BEq.beq (e₁.opt0Plus.eval s) (e₂.opt0Plus.eval s)) := sorry-- congr (congr (congrArg (not ∘ BEq.beq)) ih₁) ih₂
-          _ = [Logic| <[e₁]> ≠ <[e₂]>].opt0Plus.eval s                       := rfl
+          _ = [Logic| ‹e₁› ≠ ‹e₂›].opt0Plus.eval s                       := rfl
       | .le e₁ e₂, s =>
         have ih₁ := Arith.opt0Plus.sound e₁ s
         have ih₂ := Arith.opt0Plus.sound e₂ s
         sorry
-        -- calc [Logic| <[e₁]> ≤ <[e₂]>].eval s
+        -- calc [Logic| ‹e₁› ≤ ‹e₂›].eval s
         --   _ = (LE.le (e₁.eval s) (e₂.eval s): Bool)                   := rfl
         --   _ = (LE.le (e₁.opt0Plus.eval s) (e₂.opt0Plus.eval s): Bool) := congr (congrArg LE.le ih₁) ih₂
-        --   _ = [Logic| <[e₁]> ≤ <[e₂]>].opt0Plus.eval s                        := rfl
+        --   _ = [Logic| ‹e₁› ≤ ‹e₂›].opt0Plus.eval s                        := rfl
       | .gt e₁ e₂, s =>
         have ih₁ := Arith.opt0Plus.sound e₁ s
         have ih₂ := Arith.opt0Plus.sound e₂ s
         sorry
-        -- calc [Logic| <[e₁]> > <[e₂]>].eval s
+        -- calc [Logic| ‹e₁› > ‹e₂›].eval s
         --   _ = (GT.gt (e₁.eval s) (e₂.eval s): Bool)                   := rfl
         --   _ = (GT.gt (e₁.opt0Plus.eval s) (e₂.opt0Plus.eval s): Bool) := congr (congrArg GT.gt ih₁) ih₂
-        --   _ = [Logic| <[e₁]> > <[e₂]>].opt0Plus.eval s                        := rfl
+        --   _ = [Logic| ‹e₁› > ‹e₂›].opt0Plus.eval s                        := rfl
       | .not b, s =>
         have ih := sound b s
-        calc [Logic| ! <[b]>].eval s
+        calc [Logic| ! ‹b›].eval s
           _ = not (b.eval s)                := rfl
           _ = not (b.opt0Plus.eval s)       := congrArg not ih
-          _ = [Logic| ! <[b]> ].opt0Plus.eval s := rfl
+          _ = [Logic| ! ‹b› ].opt0Plus.eval s := rfl
       | .and b₁ b₂, s =>
         have ih₁ := sound b₁ s
         have ih₂ := sound b₂ s
-        calc [Logic| <[b₁]> && <[b₂]> ].eval s
+        calc [Logic| ‹b₁› && ‹b₂› ].eval s
           _ = and (b₁.eval s) (b₂.eval s)                   := rfl
           _ = and (b₁.opt0Plus.eval s) (b₂.opt0Plus.eval s) := congr (congrArg and ih₁) ih₂
-          _ = [Logic| <[b₁]> && <[b₂]> ].opt0Plus.eval s             := rfl
+          _ = [Logic| ‹b₁› && ‹b₂› ].opt0Plus.eval s             := rfl
 
     theorem Command.opt0Plus.sound: Command.transform_sound Command.opt0Plus
       | .skip, _, _ => ⟨id, id⟩
@@ -1449,7 +1449,7 @@ namespace SoftwareFoundations.ProgrammingLanguageFoundations.Equiv
             match n with
               | .zero => by simp_all
               | .succ _ =>
-                calc [Arith| <[num:Nat.succ _]> + <[e₂]>].eval s
+                calc [Arith| ‹num:Nat.succ _› + ‹e₂›].eval s
                   _ = (Arith.num (.succ _)).eval s + e₂.eval s                   := by rfl
                   _ = (Arith.num (.succ _)).opt0Plus.eval s + e₂.opt0Plus.eval s := by rw [ih₁, ih₂]
                   _ = (Arith.plus (.num (.succ _)) e₂).opt0Plus.eval s           := by rfl
@@ -1538,7 +1538,7 @@ namespace SoftwareFoundations.ProgrammingLanguageFoundations.Equiv
 
   example: [Arith| Y + X].subst "X" [Arith| 42 + 53] = [Arith| Y + (42 + 53)] := rfl
 
-  def Arith.subst.equiv: Prop := ∀ id₁ id₂ e₁ e₂, [Imp| <[id₁]> := <[e₁]>; <[id₂]> := <[e₂]>] ≈ [Imp| <[id₁]> := <[e₁]>; <[id₂]> := <[e₂.subst id₁ e₁]>]
+  def Arith.subst.equiv: Prop := ∀ id₁ id₂ e₁ e₂, [Imp| ‹id₁› := ‹e₁›; ‹id₂› := ‹e₂›] ≈ [Imp| ‹id₁› := ‹e₁›; ‹id₂› := ‹e₂.subst id₁ e₁›]
 
   namespace Term
     theorem Arith.subst.equiv.inequiv: ¬Arith.subst.equiv := sorry
@@ -1590,27 +1590,26 @@ namespace SoftwareFoundations.ProgrammingLanguageFoundations.Equiv
 
     syntax:50 "skip" : havoc_cmd
     syntax:50 ident ":=" arith : havoc_cmd
-    syntax:50 "<[" term "]>" ":=" arith : havoc_cmd
+    syntax:50 "‹" term "›" ":=" arith : havoc_cmd
     syntax:40 havoc_cmd ";" havoc_cmd : havoc_cmd
     syntax:50 "ite" "(" logic ")" "{" havoc_cmd "}" "else" "{" havoc_cmd "}" : havoc_cmd
     syntax:50 "while" "(" logic ")" "{" havoc_cmd "}" : havoc_cmd
     syntax:50 "havoc" ident : havoc_cmd
     syntax "(" havoc_cmd ")" : havoc_cmd
-    syntax "<[" term "]>" : havoc_cmd
+    syntax "‹" term "›" : havoc_cmd
 
     syntax "[Havoc|" havoc_cmd "]" : term
 
     macro_rules
       | `([Havoc| skip])                                => `(Command.skip)
       | `([Havoc| $id:ident := $e:arith])               => `(Command.assign $(Lean.quote (toString id.getId)) [Arith| $e])
-      | `([Havoc| <[ $t:term ]> := $e:arith])           => `(Command.assign $(Lean.quote t) [Arith| $e])
+      | `([Havoc| ‹$t:term› := $e:arith])           => `(Command.assign $(Lean.quote t) [Arith| $e])
       | `([Havoc| $x; $y])                              => `(Command.seq [Havoc| $x] [Havoc| $y])
       | `([Havoc| ite ( $c:logic ) { $t } else { $f }]) => `(Command.if [Logic| $c] [Havoc| $t] [Havoc| $f])
       | `([Havoc| while ( $c:logic ) { $b }])           => `(Command.while [Logic| $c] [Havoc| $b])
       | `([Havoc| havoc $id:ident ])                    => `(Command.havoc $(Lean.quote (toString id.getId)))
       | `([Havoc| ( $c )])                              => `([Havoc| $c])
-      | `([Havoc| <[ $t:term ]> ])                      => pure t
-
+      | `([Havoc| ‹$t:term› ])                      => pure t
 
     inductive CommandEval: Command → State → State → Prop where
       | skip {s: State}: CommandEval .skip s s
@@ -1720,7 +1719,7 @@ namespace SoftwareFoundations.ProgrammingLanguageFoundations.Equiv
   private def _root_.SoftwareFoundations.LogicalFoundations.Imp.Command.zProp (c: Command): Prop := sorry
 
   namespace Term
-    example (id₁ id₂: String) (e₁ e₂: Arith) (h₁: OccursCheck id₁ e₁) (h₂: OccursCheck id₂ e₂): [Imp| <[id₁]> := <[e₁]>; <[id₂]> := <[e₂]>] ≈ [Imp| <[id₂]> := <[e₂]>; <[id₁]> := <[e₁]>] := sorry
+    example (id₁ id₂: String) (e₁ e₂: Arith) (h₁: OccursCheck id₁ e₁) (h₂: OccursCheck id₂ e₂): [Imp| ‹id₁› := ‹e₁›; ‹id₂› := ‹e₂›] ≈ [Imp| ‹id₂› := ‹e₂›; ‹id₁› := ‹e₁›] := sorry
 
     -- TODO: For loops in Imp
 
@@ -1730,7 +1729,7 @@ namespace SoftwareFoundations.ProgrammingLanguageFoundations.Equiv
   end Term
 
   namespace Tactic
-    example (id₁ id₂: String) (e₁ e₂: Arith) (h₁: OccursCheck id₁ e₁) (h₂: OccursCheck id₂ e₂): [Imp| <[id₁]> := <[e₁]>; <[id₂]> := <[e₂]>] ≈ [Imp| <[id₂]> := <[e₂]>; <[id₁]> := <[e₁]>] := by sorry
+    example (id₁ id₂: String) (e₁ e₂: Arith) (h₁: OccursCheck id₁ e₁) (h₂: OccursCheck id₂ e₂): [Imp| ‹id₁› := ‹e₁›; ‹id₂› := ‹e₂›] ≈ [Imp| ‹id₂› := ‹e₂›; ‹id₁› := ‹e₁›] := by sorry
 
     -- TODO: For loops in Imp
 
@@ -1740,7 +1739,7 @@ namespace SoftwareFoundations.ProgrammingLanguageFoundations.Equiv
   end Tactic
 
   namespace Blended
-    example (id₁ id₂: String) (e₁ e₂: Arith) (h₁: OccursCheck id₁ e₁) (h₂: OccursCheck id₂ e₂): [Imp| <[id₁]> := <[e₁]>; <[id₂]> := <[e₂]>] ≈ [Imp| <[id₂]> := <[e₂]>; <[id₁]> := <[e₁]>] := sorry
+    example (id₁ id₂: String) (e₁ e₂: Arith) (h₁: OccursCheck id₁ e₁) (h₂: OccursCheck id₂ e₂): [Imp| ‹id₁› := ‹e₁›; ‹id₂› := ‹e₂›] ≈ [Imp| ‹id₂› := ‹e₂›; ‹id₁› := ‹e₁›] := sorry
 
     -- TODO: For loops in Imp
 
